\item Sean $U,V$ y $W$ $K$-EV. Probar que:
    \begin{enumerate}
        \item $(S+T)^t=S^t+T^t$ para $S,T\in L(U,V).$
            \begin{mdframed}[style=s]
                $(S+T)^t(g)v=g(S+T)v=gSv+gTv=(g\circ S)v+(g\circ T)v=(S^tg+T^tg)v\to (S+T)^t=S^t+T^t$
            \end{mdframed}
        \item $(\alpha T)^t=\alpha T^t$ para $\alpha\in\K$ y $T\in L(U,V)$
            \begin{mdframed}[style=s]
                $(\alpha T)^tg=g(\alpha T)=\alpha gT=\alpha T^tg\to (\alpha T)^t=\alpha T^t$
            \end{mdframed}
        \item $(ST)^t=T^tS^t$ para $S\in L(V,U)$ y $T\in (W,V)$
            \begin{mdframed}[style=s]
                $(ST)^tg=g(ST)=(g(S))T=T^tg(S)=T^tS^tg\to (ST)^t=T^tS^t$
            \end{mdframed}
    \end{enumerate}
    